Cleanup + comments

code/datatypes/cuMin.v
@@ -1,291 +1,345 @@
 Require Import maps EqNat Lists.List.
 Import ListNotations.
 
-(* Star tagged variables can only be specialized to non-functional data types,
-   while the empty tag allows this *)
+Section General.
 
-Inductive tag : Type :=
- | tag_star  : tag
- | tag_empty : tag.
-
-Inductive ty : Type :=
-  | TVar  : id -> ty
-  | TBool : ty
-  | TNat  : ty
-  | TList : ty -> ty
-  | TPair : ty -> ty -> ty
-  | TFun  : ty -> ty -> ty.
-
-Inductive context : Type := 
- | con : (partial_map tag) -> (partial_map ty) -> context.
-
-Definition empty := con emptymap emptymap.
- 
-Definition typecon (Gamma : context) : (partial_map ty) :=
-match Gamma with
- | (con _ tyc) => tyc
-end.
-
-Definition tagcon (Gamma : context) : (partial_map tag) :=
-match Gamma with
- | (con tagc _) => tagc
-end.
-
-Definition type_update (Gamma : context) (x : id) (v : ty) := 
- (con (tagcon Gamma) (update (typecon Gamma) x v)).
- 
-Definition tag_update (Gamma : context) (x : id) (v : tag) := 
- (con (update (tagcon Gamma) x v) (typecon Gamma)).
-
-Inductive tm : Type :=
-  | tvar   : id -> tm
-  | tapp   : tm -> tm -> tm
-  | tfun   : id -> list ty -> tm
-  | tlet   : tm -> tm -> tm -> tm
-  | ttrue  : tm
-  | tfalse : tm
-  | tfail  : ty -> tm
-  | tany   : ty -> tm
-  | tzero  : tm
-  | tsucc  : tm -> tm
-  | tadd   : tm -> tm -> tm
-  | teqn   : tm -> tm -> tm
-  | tpair  : tm -> tm -> tm
-  | tnil   : tm
-  | tcons  : tm -> tm -> tm
-  | tcasep : tm -> tm -> tm
-  | tcaseb : tm -> tm -> tm -> tm
-  | tcasel : tm -> tm -> tm -> tm.
-
-Inductive quantifier : Type :=
- for_all : id -> tag -> quantifier.
- 
-Definition qid (q : quantifier) : id := match q with (for_all id _) => id end.
-
-Inductive func_decl : Type :=
- FDecl : id -> list quantifier -> ty -> (list id) -> tm -> func_decl.
-
-Definition fd_qs (fd : func_decl) := match fd with FDecl _ qs _ _ _ => qs end.
-
-Fixpoint cat_options {T : Type} (l : list (option T)) : list T :=
+  (* Takes a list of option T and returns the Some values. *)
+  Fixpoint cat_options {T : Type} (l : list (option T)) : list T :=
   match l with
   | []             => []
   | (Some x) :: ls => x :: (cat_options ls)
   |  None    :: ls =>      (cat_options ls)
   end.
-
-Definition is_star_tagged (q : quantifier) : bool :=
-  match q with
-  | (for_all _ tag_star)  => true
-  | (for_all _ tag_empty) => false
-  end.
-
-Definition fd_to_tys (Gamma : context) (fd : func_decl) : (list ty) :=
-  match fd with
-  | FDecl _ [] _ _ _ => []
-  | FDecl _ qs _ _ _ => cat_options (map (fun q => typecon Gamma (qid q)) (filter is_star_tagged qs))
-  end.
-
-Definition beq_fd (fd1 fd2 : func_decl) : bool :=
-  match fd1, fd2 with
-    | (FDecl m _ _ _ _), (FDecl n _ _ _ _) => if (beq_id m n ) then true else false
-  end.
-
-Definition program := list func_decl.
-
-Definition lookup_func (p : program) (i : id) :=
- find (fun fd => match fd with (FDecl j _ _ _ _) => (beq_id i j) end) p.
-
-Reserved Notation "Gamma '|-' T '\in_data'" (at level 40).
-Inductive data : context -> ty -> Prop :=
-  | D_Var :  forall Gamma n,
-              (tagcon Gamma) n  = Some tag_star ->
-              Gamma |- (TVar n) \in_data
-  | D_Bool : forall Gamma, Gamma |- TBool \in_data
-  | D_Nat :  forall Gamma, Gamma |- TNat \in_data
-  | D_List : forall Gamma T,
-               Gamma |- T \in_data ->
-               Gamma |- (TList T) \in_data
-  | D_Pair : forall Gamma T T', 
-               Gamma |- T \in_data ->
-               Gamma |- T' \in_data ->
-               Gamma |- (TPair T T') \in_data
-where "Gamma '|-' T '\in_data'" := (data Gamma T).
-
-Fixpoint ty_subst (k: id) (t: ty) (t': ty) : ty :=
-  match t' with
-   | TVar i      =>  if (beq_id i k) then t else TVar i
-   | TBool       => TBool
-   | TNat        => TNat
-   | TList T     => TList (ty_subst k t T)
-   | TPair TF TS => TPair (ty_subst k t TF) (ty_subst k t TS)
-   | TFun  TA TR => TFun  (ty_subst k t TA) (ty_subst k t TR)
-  end.
-
-Fixpoint zip {U V : Type} (us : list U) (vs : list V) : (list (U * V)) :=
+  
+  (* Takes two lists and returns a list of pairs *)
+  Fixpoint zip {U V : Type} (us : list U) (vs : list V) : (list (U * V)) :=
   match us, vs with
    | [], _  => [] 
    | _ , [] => [] 
    | (u :: us), (v :: vs) => (u, v) :: (zip us vs)
   end.
 
-Definition multi_ty_subst (qtys : list (quantifier * ty)) (t : ty) : ty := 
- fold_right (fun qty t => match qty with (for_all id _, ty) => ty_subst id ty t end) t qtys.
-  
-Definition specialize_func (fd : func_decl) (tys : list ty) : option ty := 
-  match fd with
-   | (FDecl _ qs t _ _) => if (beq_nat (length qs) (length tys))
-                           then Some (multi_ty_subst (zip qs tys) t)
-                           else None
-  end.
+End General.
 
-Fixpoint is_concr_ty (t : ty) : Prop := 
-  match t with
-  | TVar  _     => False
-  | TList T     => is_concr_ty T
-  | TPair TF TS => (and (is_concr_ty TF) (is_concr_ty TS))
-  | TFun  TA TR => (and (is_concr_ty TA) (is_concr_ty TR))
-  | _           => True
-  end.
+  (* Data types *)
+  Inductive ty : Type :=
+    | TVar  : id -> ty
+    | TBool : ty
+    | TNat  : ty
+    | TList : ty -> ty
+    | TPair : ty -> ty -> ty
+    | TFun  : ty -> ty -> ty.
 
-Reserved Notation "Gamma '|-' t '\in' T" (at level 40).
+  (* Terms *)
+  Inductive tm : Type :=
+    | tvar   : id -> tm
+    | tapp   : tm -> tm -> tm
+    | tfun   : id -> list ty -> tm
+    | tlet   : tm -> tm -> tm -> tm
+    | ttrue  : tm
+    | tfalse : tm
+    | tfail  : ty -> tm
+    | tany   : ty -> tm
+    | tzero  : tm
+    | tsucc  : tm -> tm
+    | tadd   : tm -> tm -> tm
+    | teqn   : tm -> tm -> tm
+    | tpair  : tm -> tm -> tm
+    | tnil   : tm
+    | tcons  : tm -> tm -> tm
+    | tcasep : tm -> tm -> tm
+    | tcaseb : tm -> tm -> tm -> tm
+    | tcasel : tm -> tm -> tm -> tm.
 
-Inductive has_type : context -> tm -> ty -> Prop :=
-  | T_Var :    forall Gamma x T,
-                 (typecon Gamma) x = Some T ->
-                 Gamma |- tvar x \in T
-  | T_True :   forall Gamma, 
-                 Gamma |- ttrue \in TBool
-  | T_False :  forall Gamma,
-                 Gamma |- tfalse \in TBool
-  | T_Zero :   forall Gamma,
-                 Gamma |- tzero \in TNat
-  | T_Succ :   forall Gamma e,
-                 Gamma |- e \in TNat -> 
-                 Gamma |- (tsucc e) \in TNat
-  | T_Nil :    forall Gamma T, 
-                 Gamma |- tnil \in (TList T)
-  | T_App :    forall Gamma e1 e2 T1 T2,
-                 Gamma |- e1 \in (TFun T1 T2) ->
-                 Gamma |- e2 \in T1 ->
-                 Gamma |- (tapp e1 e2) \in T2
-  | T_Let :    forall Gamma e1 e2 x T1 T2,
-                 Gamma |- e1 \in T1 ->
-                 (type_update Gamma x T1) |- e2 \in T2 ->
-                 Gamma |- (tlet (tvar x) e1 e2) \in T2
-  | T_Fun :    forall Gamma P id fd tys T,
-                 lookup_func P id = Some fd ->
-                 specialize_func fd tys = Some T ->
-                 Forall (data Gamma) (fd_to_tys Gamma fd) ->
-                 Gamma |- (tfun id tys) \in T
-  | T_Fun2 :   forall Gamma P id fd tys T,
-                 lookup_func P id = Some fd ->
-                 length tys = length (fd_qs fd) ->
-                 specialize_func fd tys = Some T ->
-                 is_concr_ty T ->
-                 Forall (data Gamma) (fd_to_tys Gamma fd) ->
-                 Gamma |- (tfun id tys) \in T
-  | T_Add :    forall Gamma e1 e2,
-                 Gamma |- e1 \in TNat ->
-                 Gamma |- e2 \in TNat ->
-                 Gamma |- (tadd e1 e2) \in TNat
-  | T_EqN :    forall Gamma e1 e2,
-                 Gamma |- e1 \in TNat ->
-                 Gamma |- e2 \in TNat ->
-                 Gamma |- (teqn e1 e2) \in TBool
-  | T_Pair:    forall Gamma e1 e2 T1 T2,
-                 Gamma |- e1 \in T1 ->
-                 Gamma |- e2 \in T2 ->
-                 Gamma |- (tpair e1 e2) \in (TPair T1 T2)
-  | T_Cons :   forall Gamma e1 e2 T,
-                 Gamma |- e1 \in T ->
-                 Gamma |- e2 \in (TList T) -> 
-                 Gamma |- (tcons e1 e2) \in (TList T)
-  | T_CaseL :  forall Gamma e e1 e2 h t T T',
-                 Gamma |- e \in (TList T') ->
-                 Gamma |- e1 \in T ->
-                 (type_update (type_update Gamma h T') t (TList T')) |- e2 \in T ->
-                 Gamma |- (tcasel e e1 e2) \in T
-  | T_CaseP :  forall Gamma e e1 l r T T1 T2,
-                 Gamma |- e \in (TPair T1 T2) ->
-                 (type_update (type_update Gamma l T1) r T2) |- e1 \in T ->
-                 Gamma |- (tcasep e e1) \in T
-  | T_CaseB :  forall Gamma e e1 e2 T,
-                 Gamma |- e \in TBool ->
-                 Gamma |- e1 \in T ->
-                 Gamma |- e2 \in T ->
-                 Gamma |- (tcaseb e e1 e2) \in T
-  | T_Fail :   forall Gamma T,
-                 Gamma |- (tfail T) \in T
-  | T_Any :    forall Gamma T,
-                 Gamma |- T \in_data ->
-                 Gamma |- (tany T) \in T
-where "Gamma '|-' t '\in' T" := (has_type Gamma t T).
-  
+  (* Tags define the data types a type variable can be specialized to.
+     Star-tagged variables can only be specialized to non-functional data types
+     while the empty tag allows any specialization. *)
+  Inductive tag : Type :=
+    | tag_star  : tag
+    | tag_empty : tag.
+
+Section Context.
+
+  (* A context maps IDs of type variables to tags and concrete types. *)
+  Inductive context : Type := 
+    | con : (partial_map tag) -> (partial_map ty) -> context.
+
+  (* Empty context *)
+  Definition empty := con emptymap emptymap.
+
+  (* Returns type context of a context. *)
+  Definition typecon (Gamma : context) : (partial_map ty) :=
+    match Gamma with (con _ tyc) => tyc end.
+
+  (* Returns tag context of a context. *)
+  Definition tagcon (Gamma : context) : (partial_map tag) :=
+    match Gamma with (con tagc _) => tagc end.
+
+  (* Updates the ID's type in a context. *)
+  Definition type_update (Gamma : context) (x : id) (v : ty) := 
+    (con (tagcon Gamma) (update (typecon Gamma) x v)).
+
+  (* Updates the ID's tag in a context. *)
+  Definition tag_update (Gamma : context) (x : id) (v : tag) := 
+    (con (update (tagcon Gamma) x v) (typecon Gamma)).
+
+End Context.
+
+Section Functions.
+
+  (* Quantifiers assign tags to IDs of type variables and are used in
+     function declarations. *)
+  Inductive quantifier : Type :=
+    for_all : id -> tag -> quantifier.
+
+  (* Returns ID of a quantifier. *)
+  Definition qid (q : quantifier) : id := match q with (for_all id _) => id end.
+
+  (* Returns true if a quantifier has a star tag, false otherwise. *)
+  Definition is_star_tagged (q : quantifier) : bool :=
+    match q with
+    | (for_all _ tag_star)  => true
+    | (for_all _ tag_empty) => false
+    end.
+
+  (* Function declarations contain all necessary information about a function.
+     * the function's name (represented by an ID)
+     * a list of quantifiers, which represent the type variables used
+     * a (possibly polymorphic) function type
+     * a list of IDs, which represent the functions arguments
+     * the term that the function evaluates to *)
+  Inductive func_decl : Type :=
+    FDecl : id -> list quantifier -> ty -> (list id) -> tm -> func_decl.
+
+  (* Returns a function declaration's list of quantifiers. *)
+  Definition fd_qs (fd : func_decl) := match fd with FDecl _ qs _ _ _ => qs end.
+
+  (* Takes a context and function declaration and returns the type of
+     all *star-tagged* type variables according to the context. *)
+  Definition fd_to_tys (Gamma : context) (fd : func_decl) : (list ty) :=
+    match fd with
+    | FDecl _ [] _ _ _ => []
+    | FDecl _ qs _ _ _ => cat_options (map (fun q => typecon Gamma (qid q))
+                                           (filter is_star_tagged qs))
+    end.
+
+  (* Boolean equality between two function declarations. *)
+  Definition beq_fd (fd1 fd2 : func_decl) : bool :=
+    match fd1, fd2 with
+    | (FDecl m _ _ _ _), (FDecl n _ _ _ _) => if (beq_id m n ) 
+                                              then true else false
+    end.
+
+  (* A program is a list of function declarations. *)
+  Definition program := list func_decl.
+
+  (* Takes a program and ID and returns a corresponding function declaration
+     if one exists within the program.*)
+  Definition lookup_func (p : program) (i : id) : (option func_decl) :=
+    find (fun fd => match fd with (FDecl j _ _ _ _) => (beq_id i j) end) p.
+
+  (* Takes an ID and substitutes corresponding type variables with a 
+     given type t within a type t'. *)
+  Fixpoint ty_subst (k: id) (t: ty) (t': ty) : ty :=
+    match t' with
+    | TVar i      =>  if (beq_id i k) then t else TVar i
+    | TBool       => TBool
+    | TNat        => TNat
+    | TList T     => TList (ty_subst k t T)
+    | TPair TF TS => TPair (ty_subst k t TF) (ty_subst k t TS)
+    | TFun  TA TR => TFun  (ty_subst k t TA) (ty_subst k t TR)
+    end.
+
+  (* Takes a list of (quantifier,type) pairs and applies a type substitution
+     of the quantifier's ID to a type repeatedly to a given type. *)
+  Definition multi_ty_subst (qtys : list (quantifier * ty)) (t : ty) : ty := 
+    fold_right (fun qty t => match qty with (for_all id _, ty) 
+                          => ty_subst id ty t end)
+               t qtys.
+
+  (* Specializes a function declaration by applying multi_ty_subst with
+     a list of concrete types. Returns the specialized type of the function. *)
+  Definition specialize_func (fd : func_decl) (tys : list ty) : option ty := 
+    match fd with
+    | (FDecl _ qs t _ _) => if (beq_nat (length qs) (length tys))
+                            then Some (multi_ty_subst (zip qs tys) t)
+                            else None
+    end.
+
+End Functions.
+
+Section Typing.
+
+  (* Rules for being a data type *)
+  Reserved Notation "Gamma '|-' T '\is_data_type'" (at level 40).
+  Inductive is_data_type : context -> ty -> Prop :=
+    | D_Var :  forall Gamma n,
+                (tagcon Gamma) n  = Some tag_star ->
+                Gamma |- (TVar n) \is_data_type
+    | D_Bool : forall Gamma, Gamma |- TBool \is_data_type
+    | D_Nat :  forall Gamma, Gamma |- TNat \is_data_type
+    | D_List : forall Gamma T,
+                 Gamma |- T \is_data_type ->
+                 Gamma |- (TList T) \is_data_type
+    | D_Pair : forall Gamma T T', 
+                 Gamma |- T \is_data_type ->
+                 Gamma |- T' \is_data_type ->
+                 Gamma |- (TPair T T') \is_data_type
+  where "Gamma '|-' T '\is_data_type'" := (is_data_type Gamma T).
+
+  (* Typing rules *)
+  Reserved Notation "Gamma '|-' t '\in' T" (at level 40).
+  Inductive has_type : context -> tm -> ty -> Prop :=
+    | T_Var :    forall Gamma x T,
+                   (typecon Gamma) x = Some T ->
+                   Gamma |- tvar x \in T
+    | T_True :   forall Gamma, 
+                   Gamma |- ttrue \in TBool
+    | T_False :  forall Gamma,
+                   Gamma |- tfalse \in TBool
+    | T_Zero :   forall Gamma,
+                   Gamma |- tzero \in TNat
+    | T_Succ :   forall Gamma e,
+                   Gamma |- e \in TNat -> 
+                   Gamma |- (tsucc e) \in TNat
+    | T_Nil :    forall Gamma T, 
+                   Gamma |- tnil \in (TList T)
+    | T_App :    forall Gamma e1 e2 T1 T2,
+                   Gamma |- e1 \in (TFun T1 T2) ->
+                   Gamma |- e2 \in T1 ->
+                   Gamma |- (tapp e1 e2) \in T2
+    | T_Let :    forall Gamma e1 e2 x T1 T2,
+                   Gamma |- e1 \in T1 ->
+                   (type_update Gamma x T1) |- e2 \in T2 ->
+                   Gamma |- (tlet (tvar x) e1 e2) \in T2
+    | T_Fun :    forall Gamma P id fd tys T,
+                   lookup_func P id = Some fd ->
+                   specialize_func fd tys = Some T ->
+                   Forall (is_data_type Gamma) (fd_to_tys Gamma fd) ->
+                   Gamma |- (tfun id tys) \in T
+    | T_Add :    forall Gamma e1 e2,
+                   Gamma |- e1 \in TNat ->
+                   Gamma |- e2 \in TNat ->
+                   Gamma |- (tadd e1 e2) \in TNat
+    | T_EqN :    forall Gamma e1 e2,
+                   Gamma |- e1 \in TNat ->
+                   Gamma |- e2 \in TNat ->
+                   Gamma |- (teqn e1 e2) \in TBool
+    | T_Pair:    forall Gamma e1 e2 T1 T2,
+                   Gamma |- e1 \in T1 ->
+                   Gamma |- e2 \in T2 ->
+                   Gamma |- (tpair e1 e2) \in (TPair T1 T2)
+    | T_Cons :   forall Gamma e1 e2 T,
+                   Gamma |- e1 \in T ->
+                   Gamma |- e2 \in (TList T) -> 
+                   Gamma |- (tcons e1 e2) \in (TList T)
+    | T_CaseL :  forall Gamma e e1 e2 h t T T',
+                   Gamma |- e \in (TList T') ->
+                   Gamma |- e1 \in T ->
+                   (type_update 
+                     (type_update Gamma h T') t (TList T')) |- e2 \in T ->
+                   Gamma |- (tcasel e e1 e2) \in T
+    | T_CaseP :  forall Gamma e e1 l r T T1 T2,
+                   Gamma |- e \in (TPair T1 T2) ->
+                   (type_update (type_update Gamma l T1) r T2) |- e1 \in T ->
+                   Gamma |- (tcasep e e1) \in T
+    | T_CaseB :  forall Gamma e e1 e2 T,
+                   Gamma |- e \in TBool ->
+                   Gamma |- e1 \in T ->
+                   Gamma |- e2 \in T ->
+                   Gamma |- (tcaseb e e1 e2) \in T
+    | T_Fail :   forall Gamma T,
+                   Gamma |- (tfail T) \in T
+    | T_Any :    forall Gamma T,
+                   Gamma |- T \is_data_type ->
+                   Gamma |- (tany T) \in T
+  where "Gamma '|-' t '\in' T" := (has_type Gamma t T).
+
+ (* End Typing. *)
+
 Section Examples.
   Example t1 : empty |- ttrue \in TBool.
   Proof. apply T_True. Qed.
-  
+
   Definition c := (type_update empty (Id 5) TNat).
-  
+
   Example t2 : c |- (tvar (Id 5)) \in TNat.
   Proof. apply T_Var. reflexivity. Qed.
-  
-  Example t3 : empty |- (tlet (tvar (Id 5)) tzero (tadd (tsucc tzero) (tvar (Id 5)))) \in TNat.
-  Proof. apply T_Let with (T1 := TNat).
-         apply T_Zero.
-         apply T_Add.
-         apply T_Succ. apply T_Zero.
-         apply T_Var. reflexivity.
+
+  Example t3 : empty |- (tlet (tvar (Id 5)) tzero 
+                        (tadd (tsucc tzero) (tvar (Id 5)))) \in TNat.
+  Proof. 
+    apply T_Let with (T1 := TNat).
+    apply T_Zero.
+    apply T_Add.
+    apply T_Succ. apply T_Zero.
+    apply T_Var. reflexivity.
   Qed.
-  
-  Example t4 : empty |- (tcasel tnil tnil (tcons (tsucc tzero) tnil)) \in (TList TNat).
-  Proof. apply T_CaseL with (T' := TNat) (h := Id 5) (t := Id 6).
-         apply T_Nil.
-         apply T_Nil.
-         apply T_Cons.
-         apply T_Succ. apply T_Zero.
-         apply T_Nil.
+
+  Example t4 : empty |- (tcasel tnil tnil 
+                                (tcons (tsucc tzero) tnil)) \in (TList TNat).
+  Proof.
+    apply T_CaseL with (T' := TNat) (h := Id 5) (t := Id 6).
+    apply T_Nil.
+    apply T_Nil.
+    apply T_Cons.
+    apply T_Succ. apply T_Zero.
+    apply T_Nil.
   Qed.
-  
-  Example t5 : (type_update empty (Id 5) TBool) |- (tcasel (tcons ttrue tnil) tfalse (tvar (Id 5))) \in TBool.
-  Proof. apply T_CaseL with (T' := TBool) (h := Id 6) (t := Id 7).
-         apply T_Cons.
-         apply T_True.
-         apply T_Nil.
-         apply T_False.
-         apply T_Var. reflexivity.
+
+  Example t5 : (type_update empty (Id 5) TBool) |- 
+               (tcasel (tcons ttrue tnil) tfalse (tvar (Id 5))) \in TBool.
+  Proof.
+    apply T_CaseL with (T' := TBool) (h := Id 6) (t := Id 7).
+    apply T_Cons.
+    apply T_True.
+    apply T_Nil.
+    apply T_False.
+    apply T_Var. reflexivity.
   Qed.
 
   Definition aContext :=
-    type_update (type_update (type_update empty (Id 5) TNat) (Id 51) TBool) (Id 2) (TVar (Id 1)).
+    type_update 
+      (type_update 
+        (type_update empty (Id 5) TNat)
+        (Id 51) TBool)
+      (Id 2) (TVar (Id 1)).
 
   Example t6 : aContext |- tvar (Id 2) \in TVar (Id 1).
   Proof. apply T_Var. reflexivity. Qed.
-  
-  Example multi_t1 : multi_ty_subst [((for_all (Id 1) tag_empty), TNat);((for_all (Id 2) tag_empty), (TList TBool))] (TFun (TVar (Id 1)) (TFun (TVar (Id 2)) TNat)) = (TFun TNat (TFun (TList TBool) TNat)).
+
+  Example multi_t1 : multi_ty_subst 
+                     [((for_all (Id 1) tag_empty), TNat);
+                      ((for_all (Id 2) tag_empty), (TList TBool))]
+                     (TFun (TVar (Id 1)) (TFun (TVar (Id 2)) TNat)) 
+                      = (TFun TNat (TFun (TList TBool) TNat)).
   Proof. reflexivity. Qed.
-  
-  Example ty_subst1 : ty_subst (Id 1) TBool (TFun (TVar (Id 1)) (TVar (Id 1))) = TFun TBool TBool.
+
+  Example ty_subst1 : ty_subst (Id 1) TBool (TFun (TVar (Id 1)) (TVar (Id 1)))
+                      = TFun TBool TBool.
   Proof. reflexivity. Qed.
-  
-  Definition prog_fd := FDecl (Id 1) [(for_all (Id 5) tag_star)] (TFun (TVar (Id 5)) (TVar (Id 5))) [Id 1] (tvar (Id 1)).
+
+  Definition prog_fd := FDecl (Id 1) 
+                              [(for_all (Id 5) tag_star)] 
+                              (TFun (TVar (Id 5)) (TVar (Id 5))) 
+                              [Id 1] 
+                              (tvar (Id 1)).
   Definition prog := [prog_fd].
 
   Example fun1 : aContext |- (tfun (Id 1) [TNat]) \in (TFun TNat TNat).
   Proof. apply T_Fun with (P := prog) (fd := prog_fd).
-  reflexivity.
-  reflexivity.
-  simpl. apply Forall_cons. apply D_Nat. apply Forall_nil.
+    reflexivity.
+    reflexivity.
+    simpl. apply Forall_cons. apply D_Nat. apply Forall_nil.
   Qed.
-  
+
   Definition aContext2 :=
   tag_update
     (type_update
       (type_update empty (Id 3) TNat)
       (Id 4) TNat)
     (Id 0) tag_star.
-    
+
   Definition union (t1 t2: tm) : tm := tcaseb (tany TNat) t1 t2.
   Definition fun3 := FDecl (Id 1)
                        [for_all (Id 0) tag_star]
@@ -301,28 +355,11 @@ Section Examples.
                     (tvar (Id 3)))
               (tvar (Id 4)) \in TNat.
   Proof. apply T_App with (T1 := TNat). apply T_App with (T1 := TNat).
-  apply T_Fun with (P := prog3) (fd := fun3).
-  reflexivity.
-  reflexivity.
-  simpl. apply Forall_nil.
-  apply T_Var. reflexivity.
-  apply T_Var. reflexivity.
-  Qed.
-  
-  Example t8 :
-    aContext2 |- tapp
-              (tapp (tfun (Id 1)
-                          (cons (TNat) nil))
-                    (tvar (Id 3)))
-              (tvar (Id 4)) \in TNat.
-  Proof. apply T_App with (T1 := TNat). apply T_App with (T1 := TNat).
-  apply T_Fun2 with (P := prog3) (fd := fun3).
-  reflexivity.
-  reflexivity.
-  reflexivity.
-  simpl. repeat split.
-  simpl. apply Forall_nil.
-  apply T_Var. reflexivity.
-  apply T_Var. reflexivity.
+    apply T_Fun with (P := prog3) (fd := fun3).
+    reflexivity.
+    reflexivity.
+    simpl. apply Forall_nil.
+    apply T_Var. reflexivity.
+    apply T_Var. reflexivity.
   Qed.
 End Examples.
